minuska/theories/unification_interface.v
@@ -17,6 +17,13 @@ end
 .
 
 
+Fixpoint sub_app_e {Σ : StaticModel} (s : SubT) (t : TermOver Expression2) : TermOver Expression2 :=
+match s with
+| [] => t
+| (x,t')::s' => sub_app_e s' (TermOverBoV_subst_expr2 t' x t)
+end
+.
+
 Class UnificationAlgorithm
     {Σ : StaticModel}
 := {
